\documentclass{article}
\usepackage{amsmath}
\usepackage{amssymb}
\usepackage{amsfonts}
\usepackage{graphicx}
\pagestyle{empty}
\usepackage[utf8]{inputenc}
\usepackage[T1]{fontenc}
\usepackage{latexml}
\oddsidemargin 0.0in
\evensidemargin 0.0in
\textwidth 6.45in
\topmargin 0.0in
\headheight 0.0in
\headsep 0.0in
\textheight 9.0in
\usepackage{amsmath}
\newcommand{\ZZ}{\Bold{Z}}
\newcommand{\NN}{\Bold{N}}
\newcommand{\RR}{\Bold{R}}
\newcommand{\CC}{\Bold{C}}
\newcommand{\QQ}{\Bold{Q}}
\newcommand{\QQbar}{\overline{\QQ}}
\newcommand{\GF}[1]{\Bold{F}_{#1}}
\newcommand{\Zp}[1]{\ZZ_{#1}}
\newcommand{\Qp}[1]{\QQ_{#1}}
\newcommand{\Zmod}[1]{\ZZ/#1\ZZ}
\newcommand{\CDF}{\Bold{C}}
\newcommand{\CIF}{\Bold{C}}
\newcommand{\CLF}{\Bold{C}}
\newcommand{\RDF}{\Bold{R}}
\newcommand{\RIF}{\Bold{I} \Bold{R}}
\newcommand{\RLF}{\Bold{R}}
\newcommand{\CFF}{\Bold{CFF}}
\newcommand{\Bold}[1]{\mathbf{#1}}
\begin{document}
To study the incentive structure for transfer, we set\begin{align*}
  k &\to 20 \\
  K &\to 20
\end{align*}\begin{align*}
  c_a(x) &\to x^{2}\\
  p(x,y) &\to \frac{1}{4} \, x + \frac{1}{4} \, y + \frac{1}{2}\\
  C_a(x) &\to x^{2}\\
  C_g(x) &\to 0\\
  c_g(x) &\to 0
\end{align*}\begin{align*}
  c_t(x) &\to x^{2}\\
  b(x,y) &\to v x + w y\\
  C_t(x) &\to x^{2}\\
  B(x,y) &\to V x + W y
\end{align*}\iflatexml
\begin{align*}
\frac{d{X}_{{a}{0}}}{dt} &= -\frac{1}{4} \, {\left({X}_{{t}{0}}^{2} \hat{{n}}_{0} - {\left(W {X}_{{t}{0}} + V {x}_{{t}{0}}\right)} \hat{{n}}_{0} + 8 \, {X}_{{a}{0}} \hat{{n}}_{0}\right)} \hat{{N}}_{0}\\
\frac{d{X}_{{t}{0}}}{dt} &= \frac{1}{4} \, {\left(W {\left({X}_{{a}{0}} + {x}_{{a}{0}} + 2\right)} \hat{{n}}_{0} - 2 \, {\left({X}_{{a}{0}} + {x}_{{a}{0}} + 2\right)} {X}_{{t}{0}} \hat{{n}}_{0}\right)} \hat{{N}}_{0}\\
\frac{d{x}_{{a}{0}}}{dt} &= -\frac{1}{4} \, {\left(\hat{{N}}_{0} {x}_{{t}{0}}^{2} - {\left({X}_{{t}{0}} w + v {x}_{{t}{0}}\right)} \hat{{N}}_{0} + 8 \, \hat{{N}}_{0} {x}_{{a}{0}}\right)} \hat{{n}}_{0}\\
\frac{d{x}_{{t}{0}}}{dt} &= \frac{1}{4} \, {\left(\hat{{N}}_{0} {\left({X}_{{a}{0}} + {x}_{{a}{0}} + 2\right)} v - 2 \, \hat{{N}}_{0} {\left({X}_{{a}{0}} + {x}_{{a}{0}} + 2\right)} {x}_{{t}{0}}\right)} \hat{{n}}_{0}
\end{align*}
\else
\begin{dgroup*}
\begin{dmath*}
\frac{d{X}_{{a}{0}}}{dt} = -\frac{1}{4} \, {\left({X}_{{t}{0}}^{2} \hat{{n}}_{0} - {\left(W {X}_{{t}{0}} + V {x}_{{t}{0}}\right)} \hat{{n}}_{0} + 8 \, {X}_{{a}{0}} \hat{{n}}_{0}\right)} \hat{{N}}_{0}\end{dmath*}
\begin{dmath*}
\frac{d{X}_{{t}{0}}}{dt} = \frac{1}{4} \, {\left(W {\left({X}_{{a}{0}} + {x}_{{a}{0}} + 2\right)} \hat{{n}}_{0} - 2 \, {\left({X}_{{a}{0}} + {x}_{{a}{0}} + 2\right)} {X}_{{t}{0}} \hat{{n}}_{0}\right)} \hat{{N}}_{0}\end{dmath*}
\begin{dmath*}
\frac{d{x}_{{a}{0}}}{dt} = -\frac{1}{4} \, {\left(\hat{{N}}_{0} {x}_{{t}{0}}^{2} - {\left({X}_{{t}{0}} w + v {x}_{{t}{0}}\right)} \hat{{N}}_{0} + 8 \, \hat{{N}}_{0} {x}_{{a}{0}}\right)} \hat{{n}}_{0}\end{dmath*}
\begin{dmath*}
\frac{d{x}_{{t}{0}}}{dt} = \frac{1}{4} \, {\left(\hat{{N}}_{0} {\left({X}_{{a}{0}} + {x}_{{a}{0}} + 2\right)} v - 2 \, \hat{{N}}_{0} {\left({X}_{{a}{0}} + {x}_{{a}{0}} + 2\right)} {x}_{{t}{0}}\right)} \hat{{n}}_{0}
\end{dmath*}
\end{dgroup*}
\fi
Equilibrium conditions are
\iflatexml

\begin{align*}
  W = 2 \, X_{t}\\
  \mathit{Vx}_{t} = X_{t}^{2} - \mathit{WX}_{t} + 8 \, X_{a}\\
  &= -X_{t}^{2} + 8 \, X_{a}\\
  v = 2 \, x_{t}\\
  \mathit{wX}_{t} = x_{t}^{2} - \mathit{vx}_{t} + 8 \, x_{a}\\
  &= -x_{t}^{2} + 8 \, x_{a}
\end{align*}
\else
\begin{dgroup*}
  
\begin{dmath*}
  W = 2 \, X_{t}
\end{dmath*}

\begin{dmath*}
  \mathit{Vx}_{t} = X_{t}^{2} - \mathit{WX}_{t} + 8 \, X_{a}\\
  = -X_{t}^{2} + 8 \, X_{a}
\end{dmath*}

\begin{dmath*}
  v = 2 \, x_{t}
\end{dmath*}

\begin{dmath*}
  \mathit{wX}_{t} = x_{t}^{2} - \mathit{vx}_{t} + 8 \, x_{a}\\
  = -x_{t}^{2} + 8 \, x_{a}
\end{dmath*}

\end{dgroup*}
\fi
So to have all $x$ values equal to $1/2$, we set
\begin{align*}
  V &\to \frac{15}{2} \\
  w &\to \frac{15}{2} \\
  v &\to 1 \\
  W &\to 1
\end{align*}for \iflatexml
\begin{align*}
\frac{d{X}_{{a}{0}}}{dt} &= -\frac{1}{8} \, {\left(2 \, {X}_{{t}{0}}^{2} \hat{{n}}_{0} + 16 \, {X}_{{a}{0}} \hat{{n}}_{0} - {\left(2 \, {X}_{{t}{0}} + 15 \, {x}_{{t}{0}}\right)} \hat{{n}}_{0}\right)} \hat{{N}}_{0}\\
\frac{d{X}_{{t}{0}}}{dt} &= -\frac{1}{4} \, {\left(2 \, {\left({X}_{{a}{0}} + {x}_{{a}{0}} + 2\right)} {X}_{{t}{0}} \hat{{n}}_{0} - {\left({X}_{{a}{0}} + {x}_{{a}{0}} + 2\right)} \hat{{n}}_{0}\right)} \hat{{N}}_{0}\\
\frac{d{x}_{{a}{0}}}{dt} &= -\frac{1}{8} \, {\left(2 \, \hat{{N}}_{0} {x}_{{t}{0}}^{2} - \hat{{N}}_{0} {\left(15 \, {X}_{{t}{0}} + 2 \, {x}_{{t}{0}}\right)} + 16 \, \hat{{N}}_{0} {x}_{{a}{0}}\right)} \hat{{n}}_{0}\\
\frac{d{x}_{{t}{0}}}{dt} &= -\frac{1}{4} \, {\left(2 \, \hat{{N}}_{0} {\left({X}_{{a}{0}} + {x}_{{a}{0}} + 2\right)} {x}_{{t}{0}} - \hat{{N}}_{0} {\left({X}_{{a}{0}} + {x}_{{a}{0}} + 2\right)}\right)} \hat{{n}}_{0}
\end{align*}
\else
\begin{dgroup*}
\begin{dmath*}
\frac{d{X}_{{a}{0}}}{dt} = -\frac{1}{8} \, {\left(2 \, {X}_{{t}{0}}^{2} \hat{{n}}_{0} + 16 \, {X}_{{a}{0}} \hat{{n}}_{0} - {\left(2 \, {X}_{{t}{0}} + 15 \, {x}_{{t}{0}}\right)} \hat{{n}}_{0}\right)} \hat{{N}}_{0}\end{dmath*}
\begin{dmath*}
\frac{d{X}_{{t}{0}}}{dt} = -\frac{1}{4} \, {\left(2 \, {\left({X}_{{a}{0}} + {x}_{{a}{0}} + 2\right)} {X}_{{t}{0}} \hat{{n}}_{0} - {\left({X}_{{a}{0}} + {x}_{{a}{0}} + 2\right)} \hat{{n}}_{0}\right)} \hat{{N}}_{0}\end{dmath*}
\begin{dmath*}
\frac{d{x}_{{a}{0}}}{dt} = -\frac{1}{8} \, {\left(2 \, \hat{{N}}_{0} {x}_{{t}{0}}^{2} - \hat{{N}}_{0} {\left(15 \, {X}_{{t}{0}} + 2 \, {x}_{{t}{0}}\right)} + 16 \, \hat{{N}}_{0} {x}_{{a}{0}}\right)} \hat{{n}}_{0}\end{dmath*}
\begin{dmath*}
\frac{d{x}_{{t}{0}}}{dt} = -\frac{1}{4} \, {\left(2 \, \hat{{N}}_{0} {\left({X}_{{a}{0}} + {x}_{{a}{0}} + 2\right)} {x}_{{t}{0}} - \hat{{N}}_{0} {\left({X}_{{a}{0}} + {x}_{{a}{0}} + 2\right)}\right)} \hat{{n}}_{0}
\end{dmath*}
\end{dgroup*}
\fi

\end{document}
