\documentclass{article}
\usepackage{amsmath}
\usepackage{amssymb}
\usepackage{amsfonts}
\usepackage{graphicx}
\pagestyle{empty}
\usepackage[utf8]{inputenc}
\usepackage[T1]{fontenc}
\usepackage{latexml}
\oddsidemargin 0.0in
\evensidemargin 0.0in
\textwidth 6.45in
\topmargin 0.0in
\headheight 0.0in
\headsep 0.0in
\textheight 9.0in
\usepackage{amsmath}
\newcommand{\ZZ}{\Bold{Z}}
\newcommand{\NN}{\Bold{N}}
\newcommand{\RR}{\Bold{R}}
\newcommand{\CC}{\Bold{C}}
\newcommand{\QQ}{\Bold{Q}}
\newcommand{\QQbar}{\overline{\QQ}}
\newcommand{\GF}[1]{\Bold{F}_{#1}}
\newcommand{\Zp}[1]{\ZZ_{#1}}
\newcommand{\Qp}[1]{\QQ_{#1}}
\newcommand{\Zmod}[1]{\ZZ/#1\ZZ}
\newcommand{\CDF}{\Bold{C}}
\newcommand{\CIF}{\Bold{C}}
\newcommand{\CLF}{\Bold{C}}
\newcommand{\RDF}{\Bold{R}}
\newcommand{\RIF}{\Bold{I} \Bold{R}}
\newcommand{\RLF}{\Bold{R}}
\newcommand{\CFF}{\Bold{CFF}}
\newcommand{\Bold}[1]{\mathbf{#1}}
\begin{document}
To study the incentive structure for transfer, we set\begin{align*}
  c_t(x) &\to x^{2}\\
  b(x,y) &\to x + y\\
  C_t(x) &\to x^{2}\\
  B(x,y) &\to -x - y
\end{align*}\begin{align*}
  C_a(x) &\to 0\\
  p(x,y) &\to p\\
  c_a(x) &\to 0\\
  C_g(x) &\to 0\\
  c_g(x) &\to 0
\end{align*}Dynamics with transfer only:\iflatexml
\begin{align*}
\frac{d{N}_{0}}{dt} &= {\left({n}_{0} p {\left(B\left({x}_{{t}{0}}, {X}_{{t}{0}}\right) - C_{t}\left({X}_{{t}{0}}\right)\right)} - {N}_{0} + 1\right)} {N}_{0}\\
\frac{d{n}_{0}}{dt} &= {\left({N}_{0} p {\left(b\left({x}_{{t}{0}}, {X}_{{t}{0}}\right) - c_{t}\left({x}_{{t}{0}}\right)\right)} - {n}_{0} + 1\right)} {n}_{0}
\end{align*}
\else
\begin{dgroup*}
\begin{dmath*}
\frac{d{N}_{0}}{dt} = {\left({n}_{0} p {\left(B\left({x}_{{t}{0}}, {X}_{{t}{0}}\right) - C_{t}\left({X}_{{t}{0}}\right)\right)} - {N}_{0} + 1\right)} {N}_{0}\end{dmath*}
\begin{dmath*}
\frac{d{n}_{0}}{dt} = {\left({N}_{0} p {\left(b\left({x}_{{t}{0}}, {X}_{{t}{0}}\right) - c_{t}\left({x}_{{t}{0}}\right)\right)} - {n}_{0} + 1\right)} {n}_{0}
\end{dmath*}
\end{dgroup*}
\fi
Or\iflatexml
\begin{align*}
\frac{d{N}_{0}}{dt} &= -{\left({\left({X}_{{t}{0}}^{2} + {X}_{{t}{0}} + {x}_{{t}{0}}\right)} {n}_{0} p + {N}_{0} - 1\right)} {N}_{0}\\
\frac{d{n}_{0}}{dt} &= -{\left({\left({x}_{{t}{0}}^{2} - {X}_{{t}{0}} - {x}_{{t}{0}}\right)} {N}_{0} p + {n}_{0} - 1\right)} {n}_{0}
\end{align*}
\else
\begin{dgroup*}
\begin{dmath*}
\frac{d{N}_{0}}{dt} = -{\left({\left({X}_{{t}{0}}^{2} + {X}_{{t}{0}} + {x}_{{t}{0}}\right)} {n}_{0} p + {N}_{0} - 1\right)} {N}_{0}\end{dmath*}
\begin{dmath*}
\frac{d{n}_{0}}{dt} = -{\left({\left({x}_{{t}{0}}^{2} - {X}_{{t}{0}} - {x}_{{t}{0}}\right)} {N}_{0} p + {n}_{0} - 1\right)} {n}_{0}
\end{dmath*}
\end{dgroup*}
\fi
And its adaptive dynamics is\iflatexml
\begin{align*}
\frac{d{X}_{{a}{0}}}{dt} &= 0\\
\frac{d{X}_{{t}{0}}}{dt} &= {\left(\hat{{n}}_{0} p D[1]\left(B\right)\left({x}_{{t}{0}}, {X}_{{t}{0}}\right) - \hat{{n}}_{0} p D[0]\left(C_{t}\right)\left({X}_{{t}{0}}\right)\right)} \hat{{N}}_{0}\\
\frac{d{x}_{{a}{0}}}{dt} &= 0\\
\frac{d{x}_{{t}{0}}}{dt} &= {\left(\hat{{N}}_{0} p D[0]\left(b\right)\left({x}_{{t}{0}}, {X}_{{t}{0}}\right) - \hat{{N}}_{0} p D[0]\left(c_{t}\right)\left({x}_{{t}{0}}\right)\right)} \hat{{n}}_{0}
\end{align*}
\else
\begin{dgroup*}
\begin{dmath*}
\frac{d{X}_{{a}{0}}}{dt} = 0\end{dmath*}
\begin{dmath*}
\frac{d{X}_{{t}{0}}}{dt} = {\left(\hat{{n}}_{0} p D[1]\left(B\right)\left({x}_{{t}{0}}, {X}_{{t}{0}}\right) - \hat{{n}}_{0} p D[0]\left(C_{t}\right)\left({X}_{{t}{0}}\right)\right)} \hat{{N}}_{0}\end{dmath*}
\begin{dmath*}
\frac{d{x}_{{a}{0}}}{dt} = 0\end{dmath*}
\begin{dmath*}
\frac{d{x}_{{t}{0}}}{dt} = {\left(\hat{{N}}_{0} p D[0]\left(b\right)\left({x}_{{t}{0}}, {X}_{{t}{0}}\right) - \hat{{N}}_{0} p D[0]\left(c_{t}\right)\left({x}_{{t}{0}}\right)\right)} \hat{{n}}_{0}
\end{dmath*}
\end{dgroup*}
\fi
Or \iflatexml
\begin{align*}
\frac{d{X}_{{a}{0}}}{dt} &= 0\\
\frac{d{X}_{{t}{0}}}{dt} &= -{\left(2 \, {X}_{{t}{0}} \hat{{n}}_{0} p + \hat{{n}}_{0} p\right)} \hat{{N}}_{0}\\
\frac{d{x}_{{a}{0}}}{dt} &= 0\\
\frac{d{x}_{{t}{0}}}{dt} &= -{\left(2 \, \hat{{N}}_{0} p {x}_{{t}{0}} - \hat{{N}}_{0} p\right)} \hat{{n}}_{0}
\end{align*}
\else
\begin{dgroup*}
\begin{dmath*}
\frac{d{X}_{{a}{0}}}{dt} = 0\end{dmath*}
\begin{dmath*}
\frac{d{X}_{{t}{0}}}{dt} = -{\left(2 \, {X}_{{t}{0}} \hat{{n}}_{0} p + \hat{{n}}_{0} p\right)} \hat{{N}}_{0}\end{dmath*}
\begin{dmath*}
\frac{d{x}_{{a}{0}}}{dt} = 0\end{dmath*}
\begin{dmath*}
\frac{d{x}_{{t}{0}}}{dt} = -{\left(2 \, \hat{{N}}_{0} p {x}_{{t}{0}} - \hat{{N}}_{0} p\right)} \hat{{n}}_{0}
\end{dmath*}
\end{dgroup*}
\fi

\end{document}
